src/Interface_Types.v
@@ -5,7 +5,7 @@ Require Export Interface_Strings_Vars.
 (* Interface Types *)
 Record ProtocolRunRequest := 
   mkPRReq {
-    prreq_att_sesplit_evt : Attestation_Session;
+    prreq_att_sess : Attestation_Session;
     prreq_req_plc: Plc;
     prreq_Evidence: Evidence;
     prreq_term: Term;
